
General linear function = $f(x) = mx+n$

$m = \frac{\Delta y}{\Delta x} = \frac{ f(x1)-f(x0)}{x1-x0}$ 


$$  f'(x) =\lim_{h \to 0} \frac{ f(x+h)-f(x)}{h} $$





## Derivative rules



| Rule        | Formula                                                          |
| ----------- | ---------------------------------------------------------------- |
| Power       | $$\frac{d}{dx} x^n = n x^{n-1}$$                                 |
| Product     | $$\frac{d}{dx}[uv] = u'v + uv'$$                                 |
| Quotient    | $$\frac{d}{dx}\left(\frac{u}{v}\right) = \frac{u'v - uv'}{v^2}$$ |
| Chain       | $$\frac{d}{dx} f(g(x)) = f'(g(x)) \cdot g'(x)$$                  |
| exponential | $$\frac{d}{dx} e^x = e^x$$                                       |





